\documentclass[12pt]{article}
\usepackage{amsmath}  % for align* environment

\title{Arithmetic Progression Problem}
\author{SAMMETA SAIPOORNA \\
        EE23BTECH11055}
\date{}

% Define variables for the arithmetic progression
\newcommand{\initialterm}{3}
\newcommand{\commondifference}{5}
\newcommand{\targetterm}{78}

\begin{document}
\maketitle

Which term of the arithmetic progression (AP): \(3, 8, 13, 18, \ldots\) is \(78\)?

Find the term (\(k\)) when the term \(x(k)\) is equal to 78.

\section{Input Table:}
\begin{center}
\begin{tabular}{|c|c|c|}
  \hline
  \(n\) & Parameters & Description \\
  \hline
  1 & \(x(0)\) & Initial Term \\
  \hline
  2 & \(d\) & Common Difference \\
  \hline
  3 & \(x(k) \times u(k)\) & Target Term \\
  \hline
  4 & \(X(z)\) & Z-Transform \\
  \hline
\end{tabular}
\end{center}

\section{Solution:}
Let's solve the problem:
\begin{align*}
\text{Let } x(n) &= [\initialterm + (n-1)\commondifference] \times u(n) \\
\text{Given: } x(k) &= \targetterm \\
\text{Substitute values into the formula:} \\
\targetterm &= \initialterm + (k-1) \times \commondifference \\
75 &= (k-1) \times 5 \\
k &= 16
\end{align*}
Therefore, the correct term number (\(k\)) when \(x(k) = 78\) in the given AP is \(k = 16\).

\section{Z-Transform:}
Let the Z-transform of \(x(n)\) be \(X(z)\). Let \(U(z)\) be the Z-transform of \(u(n)\).
\begin{align}
X(z) &= x(0)U(z) + dz^{-1}Z\{nu(n)\} \\
&= \frac{\initialterm}{1 - z^{-1}} + \frac{\commondifference z^{-1}}{(1 - z^{-1})^2} \\
&= \frac{\initialterm(1 - z^{-1}) + \commondifference z^{-1}}{(1 - z^{-1})^2} \\
&= \frac{\initialterm - \initialterm z^{-1} + \commondifference z^{-1}}{(1 - z^{-1})^2} \\
&= \frac{\initialterm + (\commondifference - \initialterm)z^{-1}}{(1 - z^{-1})^2} \quad \text{for all } |z| > 1
\end{align}

The general form of an AP is given by \(x(n) = a + (n-1)d\),
The Z-transform of the general AP \(x(n)\) is given by:
\begin{align*}
X(z) &= \mathcal{Z}\{x(n)\} \\
&= A(z) + \frac{D(z)}{z-1}
\end{align*}
where \(A(z)\) and \(D(z)\) are the Z-transforms of \(a\) and  \(d\), respectively.

Substitute the values for the given AP \(3, 8, 13, 18, \ldots\) into this general Z-transform expression:
\begin{align*}
a &= \initialterm \\
d &= \commondifference
\end{align*}
Substituting these values:
\begin{align*}
A(z) &= \frac{\initialterm}{1 - z^{-1}} \\
D(z) &= \frac{\commondifference}{1 - z^{-1}}
\end{align*}
Now, substitute these into the general Z-transform expression:
\begin{align*}
X(z) &= \frac{\initialterm}{1 - z^{-1}} + \frac{\commondifference}{z-1} \\
X(z) &= \frac{\initialterm z}{z-1} + \frac{\commondifference}{z-1}
\end{align*}

\end{document}
